Nfp.lean
@@ -28,4 +28,6 @@ These `#print axioms` lines help ensure we only depend on a small set of axioms
 #print axioms Nfp.LocalSystem.eval_eq
 #print axioms Nfp.Circuit.eval
 #print axioms Nfp.Circuit.evalInput
+#print axioms Nfp.Circuit.Interface.eval
 #print axioms Nfp.Circuit.checkEquiv
+#print axioms Nfp.Circuit.checkEquivOnInterface
