Nfp/Circuit.lean
@@ -1,7 +1,9 @@
 -- SPDX-License-Identifier: AGPL-3.0-or-later
 
 import Nfp.Circuit.Basic
+import Nfp.Circuit.Interface
 import Nfp.Circuit.Semantics
+import Nfp.Circuit.WellFormed
 import Nfp.Circuit.Cert
 
 /-!
